code/k256/Hacl.Impl.K256.GLV.Constants.fst
@@ -1,0 +1,126 @@
+module Hacl.Impl.K256.GLV.Constants
+
+open FStar.HyperStack
+open FStar.HyperStack.ST
+open FStar.Mul
+
+open Lib.IntTypes
+open Lib.Buffer
+
+module ST = FStar.HyperStack.ST
+
+module SG = Hacl.Spec.K256.GLV
+open Hacl.K256.Field
+open Hacl.K256.Scalar
+
+#set-options "--z3rlimit 50 --fuel 0 --ifuel 0"
+
+inline_for_extraction noextract
+val make_minus_lambda: f:qelem -> Stack unit
+  (requires fun h -> live h f)
+  (ensures  fun h0 _ h1 -> modifies (loc f) h0 h1 /\
+    qas_nat h1 f == SG.minus_lambda)
+
+let make_minus_lambda f =
+  [@inline_let]
+  let x =
+   (u64 0xe0cfc810b51283cf,
+    u64 0xa880b9fc8ec739c2,
+    u64 0x5ad9e3fd77ed9ba4,
+    u64 0xac9c52b33fa3cf1f) in
+
+  assert_norm (SG.minus_lambda == qas_nat4 x);
+  make_u64_4 f x
+
+
+inline_for_extraction noextract
+val make_beta: f:felem -> Stack unit
+  (requires fun h -> live h f)
+  (ensures  fun h0 _ h1 -> modifies (loc f) h0 h1 /\
+    as_nat h1 f == SG.beta /\ inv_fully_reduced h1 f)
+
+let make_beta f =
+  [@inline_let]
+  let x =
+   (u64 0x96c28719501ee,
+    u64 0x7512f58995c13,
+    u64 0xc3434e99cf049,
+    u64 0x7106e64479ea,
+    u64 0x7ae96a2b657c) in
+
+  assert_norm (0x96c28719501ee <= max52);
+  assert_norm (0x7ae96a2b657c <= max48);
+  assert_norm (SG.beta == as_nat5 x);
+  make_u52_5 f x
+
+
+inline_for_extraction noextract
+val make_minus_b1: f:qelem -> Stack unit
+  (requires fun h -> live h f)
+  (ensures  fun h0 _ h1 -> modifies (loc f) h0 h1 /\
+    qas_nat h1 f == SG.minus_b1)
+
+let make_minus_b1 f =
+  [@inline_let]
+  let x =
+   (u64 0x6f547fa90abfe4c3,
+    u64 0xe4437ed6010e8828,
+    u64 0x0,
+    u64 0x0) in
+
+  assert_norm (SG.minus_b1 == qas_nat4 x);
+  make_u64_4 f x
+
+
+inline_for_extraction noextract
+val make_minus_b2: f:qelem -> Stack unit
+  (requires fun h -> live h f)
+  (ensures  fun h0 _ h1 -> modifies (loc f) h0 h1 /\
+    qas_nat h1 f == SG.minus_b2)
+
+let make_minus_b2 f =
+  [@inline_let]
+  let x =
+   (u64 0xd765cda83db1562c,
+    u64 0x8a280ac50774346d,
+    u64 0xfffffffffffffffe,
+    u64 0xffffffffffffffff) in
+
+  assert_norm (SG.minus_b2 == qas_nat4 x);
+  make_u64_4 f x
+
+
+inline_for_extraction noextract
+val make_g1: f:qelem -> Stack unit
+  (requires fun h -> live h f)
+  (ensures  fun h0 _ h1 -> modifies (loc f) h0 h1 /\
+    qas_nat h1 f == SG.g1)
+
+let make_g1 f =
+  [@inline_let]
+  let x =
+   (u64 0xe893209a45dbb031,
+    u64 0x3daa8a1471e8ca7f,
+    u64 0xe86c90e49284eb15,
+    u64 0x3086d221a7d46bcd) in
+
+  assert_norm (SG.g1 == qas_nat4 x);
+  make_u64_4 f x
+
+
+inline_for_extraction noextract
+val make_g2: f:qelem -> Stack unit
+  (requires fun h -> live h f)
+  (ensures  fun h0 _ h1 -> modifies (loc f) h0 h1 /\
+    qas_nat h1 f == SG.g2)
+
+let make_g2 f =
+  [@inline_let]
+  let x =
+   (u64 0x1571b4ae8ac47f71,
+    u64 0x221208ac9df506c6,
+    u64 0x6f547fa90abfe4c4,
+    u64 0xe4437ed6010e8828) in
+
+  assert_norm (SG.g2 == qas_nat4 x);
+  make_u64_4 f x
