code/k256/Hacl.Impl.K256.GLV.fst
@@ -1,0 +1,174 @@
+module Hacl.Impl.K256.GLV
+
+open FStar.HyperStack
+open FStar.HyperStack.ST
+open FStar.Mul
+
+open Lib.IntTypes
+open Lib.Buffer
+
+module ST = FStar.HyperStack.ST
+module LSeq = Lib.Sequence
+
+module BE = Hacl.Impl.Exponentiation
+module ME = Hacl.Impl.MultiExponentiation
+module PM = Hacl.Impl.K256.PointMul
+
+module S = Spec.K256
+module SG = Hacl.Spec.K256.GLV
+module SGL = Hacl.Spec.K256.GLV.Lemmas
+
+open Hacl.K256.Field
+open Hacl.K256.Scalar
+open Hacl.Impl.K256.Point
+
+open Hacl.Impl.K256.GLV.Constants
+
+#set-options "--z3rlimit 50 --fuel 0 --ifuel 0"
+
+
+inline_for_extraction noextract
+val scalar_split_lambda_g1g2 (tmp1 tmp2 k1 k2 k: qelem) : Stack unit
+  (requires fun h ->
+    live h k /\ live h k1 /\ live h k2 /\
+    live h tmp1 /\ live h tmp2 /\
+    disjoint k k1 /\ disjoint k k2 /\ disjoint k1 k2 /\
+    disjoint tmp1 k1 /\ disjoint tmp1 k2 /\ disjoint tmp1 k /\
+    disjoint tmp2 k1 /\ disjoint tmp2 k2 /\ disjoint tmp2 k /\
+    disjoint tmp1 tmp2 /\ qas_nat h k < S.q)
+  (ensures  fun h0 _ h1 ->
+    modifies (loc k1 |+| loc k2 |+| loc tmp1 |+| loc tmp2) h0 h1 /\
+   (let k1 = qas_nat h1 k1 in let k2 = qas_nat h1 k2 in
+    k1 < S.q /\ k1 = SG.qmul_shift_384 (qas_nat h0 k) SG.g1 /\
+    k2 < S.q /\ k2 = SG.qmul_shift_384 (qas_nat h0 k) SG.g2))
+
+let scalar_split_lambda_g1g2 tmp1 tmp2 k1 k2 k =
+  make_g1 tmp1; // tmp1 = g1
+  make_g2 tmp2; // tmp2 = g2
+  qmul_shift_384 k1 k tmp1; // k1 = c1 = qmul_shift_384 k g1
+  qmul_shift_384 k2 k tmp2; // k2 = c2 = qmul_shift_384 k g2
+  let h0 = ST.get () in
+  SG.qmul_shift_384_lemma (qas_nat h0 k) (qas_nat h0 tmp1);
+  SG.qmul_shift_384_lemma (qas_nat h0 k) (qas_nat h0 tmp2);
+  assert (qas_nat h0 k1 < S.q /\ qas_nat h0 k2 < S.q)
+
+
+val scalar_split_lambda (k1 k2 k: qelem) : Stack unit
+  (requires fun h ->
+    live h k /\ live h k1 /\ live h k2 /\
+    disjoint k k1 /\ disjoint k k2 /\ disjoint k1 k2 /\
+    qas_nat h k < S.q)
+  (ensures  fun h0 _ h1 -> modifies (loc k1 |+| loc k2) h0 h1 /\
+   (let k1_s, k2_s = SG.scalar_split_lambda (qas_nat h0 k) in
+    let k1 = qas_nat h1 k1 in let k2 = qas_nat h1 k2 in
+    k1 < S.q /\ k1 == k1_s /\ k2 < S.q /\ k2 == k2_s /\
+    k1 < pow2 129 /\ k2 < pow2 129))
+
+[@CInline]
+let scalar_split_lambda k1 k2 k =
+  let h0 = ST.get () in
+  SGL.lemma_scalar_split_lambda_fits (qas_nat h0 k);
+  push_frame ();
+  let tmp1 = create_qelem () in
+  let tmp2 = create_qelem () in
+  scalar_split_lambda_g1g2 tmp1 tmp2 k1 k2 k;
+
+  make_minus_b1 tmp1; // tmp1 = minus_b1
+  make_minus_b2 tmp2; // tmp2 = minus_b2
+  qmul k1 k1 tmp1; // k1 = c1 = c1 * minus_b1
+  qmul k2 k2 tmp2; // k2 = c2 = c2 * minus_b2
+
+  make_minus_lambda tmp1; // tmp1 = minus_lambda
+  qadd k2 k1 k2; // k2 = r2 = c1 + c2
+  qmul tmp2 k2 tmp1; // tmp2 = r2 * minus_lambda
+  qadd k1 k tmp2; // k1 = r1 = k + r2 * minus_lambda
+  pop_frame ()
+
+
+// [lambda]P
+inline_for_extraction noextract
+val point_mul_lambda: res:point -> p:point -> Stack unit
+  (requires fun h ->
+    live h res /\ live h p /\ eq_or_disjoint res p /\
+    point_inv h p)
+  (ensures  fun h0 _ h1 -> modifies (loc res) h0 h1 /\
+    point_inv h1 res /\
+    point_eval h1 res == SG.point_mul_lambda (point_eval h0 p))
+
+let point_mul_lambda res p =
+  push_frame ();
+  let rx, ry, rz = getx res, gety res, getz res in
+  let px, py, pz = getx p, gety p, getz p in
+  let beta = create_felem () in
+  make_beta beta;
+  fmul rx beta px;
+
+  copy_felem ry py;
+  copy_felem rz pz;
+  pop_frame ()
+
+
+// TODO: set it to a constant?
+// [lambda]G
+inline_for_extraction noextract
+val point_mul_g_lambda: res:point -> Stack unit
+  (requires fun h -> live h res)
+  (ensures  fun h0 _ h1 -> modifies (loc res) h0 h1 /\
+    point_inv h1 res /\
+    point_eval h1 res == SG.point_mul_g_lambda ())
+
+let point_mul_g_lambda res =
+  push_frame ();
+  let g = create_point () in
+  PM.make_g g;
+  point_mul_lambda res g;
+  pop_frame ()
+
+
+// TODO: share a table [0; P; 2P; ..; 15P] between P and ([lambda]P)
+val point_mul_split_lambda: out:point -> scalar:qelem -> q:point -> Stack unit
+  (requires fun h ->
+    live h out /\ live h scalar /\ live h q /\
+    disjoint out q /\ disjoint out scalar /\ disjoint q scalar /\
+    point_inv h q /\ qas_nat h scalar < S.q)
+  (ensures  fun h0 _ h1 -> modifies (loc out) h0 h1 /\
+    point_inv h1 out /\
+    point_eval h1 out == S.point_mul (qas_nat h0 scalar) (point_eval h0 q))
+
+[@CInline]
+let point_mul_split_lambda out scalar q =
+  let h0 = ST.get () in
+  push_frame ();
+  let q2 = create_point () in
+  point_mul_lambda q2 q;
+
+  let r1 = create_qelem () in
+  let r2 = create_qelem () in
+  scalar_split_lambda r1 r2 scalar;
+
+  PM.make_point_at_inf out;
+  ME.lexp_double_fw_vartime 15ul 0ul PM.mk_k256_concrete_ops (null uint64)
+    q 4ul 129ul r1 q2 r2 out 4ul;
+
+  assume (
+    SGL.point_mul_split_lambda (qas_nat h0 scalar) (point_eval h0 q) ==
+    S.point_mul (qas_nat h0 scalar) (point_eval h0 q));
+  pop_frame ()
+
+
+// TODO: precompute a table [0; G; 2G; ..; 15G]?
+val point_mul_g_split_lambda: out:point -> scalar:qelem -> Stack unit
+  (requires fun h ->
+    live h out /\ live h scalar /\ disjoint out scalar /\
+    qas_nat h scalar < S.q)
+  (ensures  fun h0 _ h1 -> modifies (loc out) h0 h1 /\
+    point_inv h1 out /\
+    point_eval h1 out == S.point_mul_g (qas_nat h0 scalar))
+
+[@CInline]
+let point_mul_g_split_lambda out scalar =
+  push_frame ();
+  let g = create 15ul (u64 0) in
+  PM.make_g g;
+  point_mul_split_lambda out scalar g;
+  pop_frame ()
